theories/program_logic/evaluation.v
@@ -155,11 +155,14 @@ End state_op.
 Section heap_op.
   Context {V A B: Type}.
 
+  Definition modifyS'' (n: nat) (f: heap V -> heap V): state V A () :=
+    State $ λ h ts, if decide (is_Some (h !! n)) then Here (tt, f h, ts) else ProgErr.
+
   Definition get (n: nat): state V A V :=
     get_heap ≫= λ h, lift_error $ into_prog $ lookup n h.
 
   Definition put (n: nat) (x : V) : state V A unit :=
-    modifyS <[n := x]>.
+    modifyS'' n  <[n := x]>.
 
   Definition alloc (v: V) : state V A nat :=
     modifyS' $ λ st, 
@@ -167,11 +170,10 @@ Section heap_op.
                 in (l, <[l:= v]> st).
 
   Definition free (n: nat): state V A unit :=
-    modifyS $ delete n.
+   modifyS'' n (delete n).
 
   Definition cmpXchg {cmp: EqDecision V} (l: nat) (v1 v2: V): state V A (V * bool) :=
     get l ≫= λ vl, if decide (vl = v1) then put l v2 ;; mret (vl, true) else mret (vl, false).
-
 End heap_op.
 
 Definition step_vis {V R T A} {cmp: EqDecision V} (c: envE V T):
