theories/program_logic/delaywp.v
@@ -314,10 +314,11 @@ Section delay_wp_heap.
     points_to γ n v -∗ (points_to γ n v' -∗ Ψ tt) -∗ wp (state_interp γ) (put n v') Ψ.
   Proof.
     iIntros "Hpt Hpost".
-    iApply wp_modifyS.
     iIntros (σ) "Hsi". 
-    iMod (si_put with "Hsi Hpt") as "($ & Hup)". 
-    by iApply "Hpost".
+    iDestruct (si_get with "Hsi Hpt") as %Hsome.
+    iMod (si_put with "Hsi Hpt") as "(? & Hup)".
+    iModIntro. simpl. rewrite Hsome. simpl. iApply wp_delay_return.
+    iFrame. by iApply "Hpost".
   Qed. 
 
   Lemma wp_alloc v (Ψ: nat -> iProp Σ):
@@ -332,10 +333,12 @@ Section delay_wp_heap.
   Lemma wp_free v l (Ψ: unit -> iProp Σ):
     points_to γ l v -∗ Ψ tt -∗ wp (state_interp γ) (free l) Ψ.
   Proof.
-    iIntros "Hpt Hpost". iApply wp_modifyS.
+    iIntros "Hpt Hpost".
     iIntros (σ) "Hsi".
-    iMod (si_free with "Hsi Hpt") as "$".
-    done.
+    iDestruct (si_get with "Hsi Hpt") as %Hsome.
+    iMod (si_free with "Hsi Hpt") as "? /=".
+    iModIntro. rewrite Hsome. simpl. iApply wp_delay_return.
+    iFrame.
   Qed.
 End delay_wp_heap.
 
