theories/program_logic/itreewp.v
@@ -747,13 +747,15 @@ Section adequacy.
       + simpl. destruct H as (Hlookup & Heq). rewrite Hlookup. subst h. simpl.
         iExists []. rewrite right_id_L.
         iFrame. auto.
-      + simpl. destruct H as (Hlookup & Heq). subst σ'. destruct v.
+      + simpl. destruct H as ((v' & Hsome) & Heq). subst σ'. destruct v.
+        rewrite Hsome. simpl.
         iExists []. rewrite right_id_L.
         iFrame. auto.
       + simpl. destruct H as (Hlookup & Heq). subst σ' v.
         iExists []. rewrite right_id_L.
         iFrame. auto.
-      + simpl. destruct H as (Hlookup & Heq). subst σ'. destruct v.
+      + simpl. destruct H as ((v' & Hsome) & Heq). subst σ'. destruct v.
+        rewrite Hsome. simpl.
         iExists []. rewrite right_id_L.
         iFrame. auto.
       + destruct v as [vret [|]]; simpl in H.
@@ -762,6 +764,7 @@ Section adequacy.
         simpl.
         rewrite HLookup. simpl.
         rewrite decide_True //. simpl.
+        rewrite HLookup.
         iExists []. rewrite right_id_L.
         iFrame. auto.
         * destruct H as (x & HLookup & -> & -> & Hneq).
